Inline top level theorem instantiated with bounds

theories/L6_PCPS/bounds.v
@@ -15,14 +15,14 @@ Section Bounds.
 
   (* ***** Fuel ***** *)
   
-  Program Instance fuel_res_pre : @resource fin nat :=
+  Global Program Instance fuel_res_pre : @resource fin nat :=
     { zero := 0;
       one_i fin := 1;
       plus x y  := x + y; }.
   Solve Obligations with (simpl; lia).
 
 
-  Program Instance fuel_res_ordered : @ordered fin nat fuel_res_pre :=
+  Global Program Instance fuel_res_ordered : @ordered fin nat fuel_res_pre :=
     { lt := Peano.lt }.
   Solve Obligations with (intro; intros; simpl; lia).
   Solve Obligations with (simpl; lia).
@@ -30,15 +30,15 @@ Section Bounds.
     destruct (lt_dec x y); auto. right. eexists (x - y). lia.
   Qed.
   
-  Program Instance fuel_res_ones : @resource_ones fin nat fuel_res_pre. 
+  Global Program Instance fuel_res_ones : @resource_ones fin nat fuel_res_pre. 
 
-  Program Instance fuel_res_hom : @nat_hom fin nat fuel_res_pre :=
+  Global Program Instance fuel_res_hom : @nat_hom fin nat fuel_res_pre :=
     { to_nat y := y }.
 
-  Program Instance fuel_res_exp : @exp_resource nat :=
+  Global Program Instance fuel_res_exp : @exp_resource nat :=
     { HRes := fuel_res_pre }.
   
-  Instance fuel_res : @fuel_resource nat.
+  Global Instance fuel_res : @fuel_resource nat.
   Proof.
     econstructor.
     eapply fuel_res_ordered.
@@ -50,7 +50,7 @@ Section Bounds.
   (* ***** Trace ***** *)
 
   
-  Program Instance trace_res_pre : @resource fin (nat * nat) :=
+  Global Program Instance trace_res_pre : @resource fin (nat * nat) :=
     { zero := (0, 0);
       one_i fin :=
         match fin with
@@ -65,10 +65,10 @@ Section Bounds.
   Next Obligation. simpl. f_equal; lia. Qed.
   Next Obligation. simpl. f_equal; lia. Qed.  
 
-  Program Instance trace_res_exp : @exp_resource (nat * nat) :=
+  Global Program Instance trace_res_exp : @exp_resource (nat * nat) :=
     { HRes := trace_res_pre }.
   
-  Instance trace_res : @trace_resource (nat * nat).
+  Global Instance trace_res : @trace_resource (nat * nat).
   Proof.
     econstructor. eapply trace_res_exp.
   Defined.
@@ -94,7 +94,7 @@ Section Bounds.
       try unfold HRexp_f in *; try unfold fuel_res in *; try unfold fuel_res_exp in *; try unfold fuel_res_pre in *;
       try unfold HRexp_t in *; try unfold trace_res in *; try unfold trace_res_exp in *; try unfold trace_res_pre in *.
 
-    Instance inline_bound_compat L G (Hi : L <= G) (Hg : G > 0):
+    Instance inline_bound_compat L G (Hi : L <= G) :
       Post_properties cenv (inline_bound L G) (inline_bound L G) (inline_bound G G). 
     Proof.
       constructor; (try (intro; intros; intro; intros; destruct cout1; destruct cout2;
@@ -161,43 +161,23 @@ Section Bounds.
     Qed.
 
     (* bound for inlining, toplevel *)
-    Definition inline_bound_top (L G : nat) : @PostT nat (nat * nat) := 
+    Definition inline_bound_top (G : nat) : @PostT nat (nat * nat) := 
       fun '(e1, rho1, c1, (t1, tapp1)) '(e2, rho2, c2, (t2, tapp2)) =>
-        c1 <= G * c2 + L.
+        let A := 1 + 2 * G + 2 * G * 2 * G in
+        c1 <= A * c2 + A.
 
-    Lemma inline_bound_top_impl (G L : nat) :
-      inclusion _ (inline_bound L G)
-                (inline_bound_top (2 * L * 2 * G + 2 * L) (1 + 2 * G + 2 * G * 2 * G)).
+    Lemma inline_bound_top_impl (G : nat) :
+      inclusion _ (inline_bound G G) (inline_bound_top G).
     Proof.
       intros [[[? ?] ?] [? ?]] [[[? ?] ?] [? ?]]. unfold inline_bound, inline_bound_top in *. unfold_all.
       intros. destructAll.
-      rewrite !NPeano.Nat.mul_add_distr_l in *. 
-      rewrite !NPeano.Nat.mul_add_distr_r in *. 
       eapply le_trans. eassumption.
       eapply le_trans. eapply plus_le_compat_r. eapply plus_le_compat_l. eapply mult_le_compat_l. eassumption.
       lia.
     Qed.
-    
-    (* Lemma inline_bound_post_inline G : *)
-    (*   post_inline cenv (inline_bound_top G) (inline_bound_top G) (inline_bound_top (3 * G)). *)
-    (* Proof. *)
-    (*   intro; intros. unfold inline_bound in *. unfold_all; simpl in *. *)
-    (*   destruct cout1; destruct cout2. destruct cout3; destruct cout4. *)
-    (*   destruct cout1'; destruct cout3'. *)
-    (*   simpl in *. *)
-    (*   inv H3; inv H4; destructAll; inv H8; inv H4; *)
-    (*     try (simpl in *; lia). *)
-    (* Qed. *)
-
-    (* Lemma inline_bound_post_inline_OOT G : *)
-    (*   post_inline_OOT (inline_bound_top G) (inline_bound_top G). *)
-    (* Proof. *)
-    (*   intro; intros. unfold inline_bound in *. unfold_all; simpl in *. *)
-    (*   destruct cout1; destruct cout3; destruct cout3'. *)
-    (*   inv H1; destructAll; inv H3; lia. *)
-    (* Qed. *)
 
   
-End Bounds.
+  End Inline_bound.
 
+End Bounds.
   
